\documentclass[fleqn]{article}
\usepackage[utf8]{inputenc}
\usepackage[pdftex]{graphicx}
\usepackage{grffile}
\usepackage{float}
\usepackage{amsmath}
\usepackage{amssymb}
\usepackage[margin=1.25in]{geometry}
\usepackage{subfig} 
\usepackage{bm}
\usepackage{algorithm}
\usepackage[noend]{algpseudocode}

\title{Assignment 5}
\author{Vishal Kumar, MIT2019090}
\date{}

\begin{document}

\maketitle
\section*{Question}
{\bf Discuss Quasi-Newton Condition with DFP and BFGS updates.}
\\
{\bf Ans. -}
\\
Newton’s method for finding an extreme point is:
\begin{align*}
x_{+} = x - H^{-1}(x)g(x)
\end{align*}
Quasi-Newton methods repeat updates of the form:
\begin{align*}
x_{+} = x + ts
\end{align*}
where, s is defined by linear system:
\begin{align*}
H(x)s = -g(x)
\end{align*}
Where, H(x) is hessian and g(x) is gradient of f.
\\
\\
{\bf Algorithm:}
\begin{algorithmic}
\State Let \quad x $\in$ R, H $>$ 0 for k=1,2,3.,.,. 
\State Repeat

\State \quad Solve\quad $H^{k-1}s^{k-1}$ = -$g^{k-1}$

\State \quad Update\quad $x^{k}$ = $x^{k-1}$ + $t_{k}s^{k-1}$

\State \quad Compute\quad $H^{k}$ from $H^{k-1}$
\end{algorithmic}
Different Quasi-Newton methods implement Step 3 differently. As
we will see, commonly we can compute:
$(H^{k})^{-1}$ from $(H^{k-1})^{-1}$
\\
\\
{\bf Davidon-Fletcher-Powell (DFP) update:}
\\
In this method, they used inverse C:
\begin{align*}
C_{+} = C + auu^{T} + bvv^{T}
\end{align*}
Multiplying by y, using the secant equation s = $C_{+}y$, and solving for a, b, yields:
\begin{align*}
C_{+} = C - \frac{Cyy^{T}C}{y^{T}Cy} + \frac{ss^{T}}{y^{T}s}
\end{align*}
then It shows:
\begin{align*}
H^{k} = (I - \frac{ys^{T}}{y^{T}s}) H^{k-1} (I - \frac{sy^{T}}{y^{T}s}) + \frac{yy^{T}}{y^{T}s}
\end{align*}
This is the Davidon-Fletcher-Powell (DFP) update.
\\
O($n^{2}$), preserves positive definiteness.
\\
{\bf Broyden-Fletcher-Goldfarb-Shanno(BFGS) update:}
\\
Let’s now try a rank-two update:
\begin{align*}
H^{k} = H^{k-1} + auu^{T} + bvv^{T}
\end{align*}
The secant equation y = $H^{k}s$ yields
\begin{align*}
y - H^{k}s = (au^{T}s)u + (bv^{T}s)v
\end{align*}
Putting u = y, v = $H^{k-1}s$, and solving for a, b we get:
\begin{align*}
H^{k} = H^{k-1} - \frac{H^{k-1}ss^{T}H^{k-1}}{s^{T}H^{k-1}s} + \frac{yy^{T}}{y^{T}s}
\end{align*}
called the Broyden-Fletcher-Goldfarb-Shanno (BFGS) update.
\\
Importantly, BFGS update preserves positive definiteness
\end{document}
